Finish proving internal versions of adequacy theorems.
The new versions allow the 'crash invariant' to be an Iris propositions,
whereas the previous versions required them to be pure Coq propositions.
The difference amounted to doing the inductive reasoning about
the repeated sequences of crashes at the meta-Coq level or 'inside' the
separation logic.

Soundness for the latter was trickier to prove (but will be easier to use)
because the proof involves counting the sum of the steps taken
by the initial program and all of the partial executions of recovery.

src/CSL/Adequacy.v
@@ -146,6 +146,24 @@ Proof.
   iModIntro; iNext; iMod "H" as ">?". by iApply IH.
 Qed.
 
+Lemma bupd_iter_mono n P Q :
+  (P -∗ Q) -∗ Nat.iter n (λ P, |==> ▷ P)%I P -∗ Nat.iter n (λ P, |==> ▷ P)%I Q.
+Proof.
+  iIntros "HPQ". iInduction n as [|n IH] "IH".
+  - simpl. iApply "HPQ".
+  - simpl. iIntros "Hiter". iMod "Hiter". iModIntro. iNext. iApply ("IH" with "HPQ Hiter").
+Qed.
+
+Lemma wptp_steps_state_inv {T} s n e1 t1 t2 σ1 σ2 Φ :
+  bind_rep_n n (Λ.(exec_pool)) (existT T e1 :: t1) σ1 (Val σ2 t2) →
+  world σ1 ∗ WP e1 @ s; ⊤ {{ Φ }} ∗ wptp s t1 ⊢
+  Nat.iter (S n) (λ P, |==> ▷ P) (world σ2).
+Proof.
+  iIntros (?) "H". iPoseProof (wptp_steps with "H") as "H"; eauto.
+  iApply (bupd_iter_mono with "[] H"); eauto.
+  iIntros "H". iDestruct "H" as (??) "(?&?&?)"; iFrame.
+Qed.
+
 Lemma bupd_iter_laterN_mono n P Q `{!Plain Q} :
   (P ⊢ Q) → Nat.iter n (λ P, |==> ▷ P)%I P ⊢ ▷^n Q.
 Proof.
@@ -210,9 +228,9 @@ Proof.
 Qed.
 End adequacy.
 
-Theorem wp_strong_adequacy {T} OpT Σ Λ `{invPreG Σ} s (e: proc OpT T) σ φ :
+Theorem wp_strong_adequacy {T} OpT Σ Λ `{invPreG Σ} s (e: proc OpT T) σ φ k:
   (∀ `{Hinv : invG Σ},
-     (|={⊤}=> ∃ stateI : State Λ → iProp Σ,
+     Nat.iter k (λ P, |==> ▷ P)%I (|={⊤}=> ∃ stateI : State Λ → iProp Σ,
        let _ : irisG OpT Λ Σ := IrisG _ _ _ Hinv stateI in
        stateI σ ∗ WP e @ s; ⊤ {{ v, ∀ σ, stateI σ ={⊤,∅}=∗ ⌜φ v σ⌝ }})%I) →
   adequate s e σ φ.
@@ -230,9 +248,14 @@ Proof.
     subst.
     cut (∃ v0 : T, existT T (@of_val OpT _ v0) = existT T' (of_val v) ∧ φ v0 σ').
     { intros (vnew&?&?). exists vnew; split; auto. inversion H0. congruence. }
-    eapply (soundness (M:=iResUR Σ) _ (S (S n))).
+    eapply (soundness (M:=iResUR Σ) _ (S k + S (S n))).
+    rewrite laterN_plus.
+    iApply bupd_iter_laterN_mono; first by reflexivity.
     iMod wsat_alloc as (Hinv) "[Hw HE]". specialize (Hwp _).
-    rewrite {1}uPred_fupd_eq in Hwp; iMod (Hwp with "[$Hw $HE]") as ">(Hw & HE & Hwp)".
+    iModIntro. iNext.
+    iApply (bupd_iter_mono k with "[Hw HE] []"); last by iApply Hwp.
+    iIntros "Hwp". rewrite {1}uPred_fupd_eq.
+    iMod ("Hwp" with "[$Hw $HE]") as ">(Hw & HE & Hwp)".
     iDestruct "Hwp" as (Istate) "[HI Hwp]".
     iApply (@wptp_result _ _ _ (IrisG _ _ _ Hinv Istate)); eauto with iFrame.
   - destruct s; last done.
@@ -246,30 +269,38 @@ Proof.
     apply exec_pool_equiv_alt_err in Hexec.
     inversion Hexec; subst; try congruence.
     cut (@non_errorable _ _ Λ e1 σ2); eauto.
-    eapply (soundness (M:=iResUR Σ) _ (S (S n'))).
+    eapply (soundness (M:=iResUR Σ) _ (S k + S (S n'))).
+    rewrite laterN_plus.
+    iApply bupd_iter_laterN_mono; first by reflexivity.
     iMod wsat_alloc as (Hinv) "[Hw HE]". specialize (Hwp _).
-    rewrite uPred_fupd_eq in Hwp; iMod (Hwp with "[$Hw $HE]") as ">(Hw & HE & Hwp)".
+    iModIntro. iNext.
+    iApply (bupd_iter_mono k with "[Hw HE] []"); last by iApply Hwp.
+    iIntros "Hwp". rewrite {1}uPred_fupd_eq.
+    iMod ("Hwp" with "[$Hw $HE]") as ">(Hw & HE & Hwp)".
     iDestruct "Hwp" as (Istate) "[HI Hwp]".
     iApply (@wptp_safe _ _ _ (IrisG _ _ _ Hinv Istate)); eauto with iFrame.
     set_solver+.
 Qed.
 
-Theorem wp_adequacy {T} OpT Σ Λ `{invPreG Σ} s (e: proc OpT T) σ φ :
+Theorem wp_adequacy {T} OpT Σ Λ `{invPreG Σ} s (e: proc OpT T) σ φ k:
   (∀ `{Hinv : invG Σ},
-     (|={⊤}=> ∃ stateI : State Λ → iProp Σ,
+     Nat.iter k (λ P, |==> ▷ P)%I (|={⊤}=> ∃ stateI : State Λ → iProp Σ,
        let _ : irisG OpT Λ Σ := IrisG _ _ _ Hinv stateI in
        stateI σ ∗ WP e @ s; ⊤ {{ v, ⌜φ v⌝ }})%I) →
   adequate s e σ (λ v _, φ v).
 Proof.
-  intros Hwp. apply (wp_strong_adequacy _ _)=> Hinv.
-  iMod Hwp as (stateI) "[Hσ H]". iExists stateI. iIntros "{$Hσ} !>".
+  intros Hwp. apply (wp_strong_adequacy _ _ _ _ _ k)=> Hinv.
+  iPoseProof (Hwp _) as "Hwp".
+  iApply (bupd_iter_mono with "[] Hwp").
+  iIntros "Hwp'".
+  iMod "Hwp'" as (stateI) "[Hσ H]". iExists stateI. iIntros "{$Hσ} !>".
   iApply (wp_wand with "H"). iIntros (v ? σ') "_".
   iMod (fupd_intro_mask' ⊤ ∅) as "_"; auto.
 Qed.
 
-Theorem wp_invariance {T} OpT Σ Λ `{invPreG Σ} s (e: proc OpT T) σ1 t2 σ2 φ :
+Theorem wp_invariance {T} OpT Σ Λ `{invPreG Σ} s (e: proc OpT T) σ1 t2 σ2 φ k:
   (∀ `{Hinv : invG Σ},
-     (|={⊤}=> ∃ stateI : State Λ → iProp Σ,
+     Nat.iter k (λ P, |==> ▷ P)%I (|={⊤}=> ∃ stateI : State Λ → iProp Σ,
        let _ : irisG OpT Λ Σ := IrisG _ _ _ Hinv stateI in
        stateI σ1 ∗ WP e @ s; ⊤ {{ _, True }} ∗ (stateI σ2 ={⊤,∅}=∗ ⌜φ⌝))%I) →
   Λ.(exec_partial) e σ1 (Val σ2 t2) →
@@ -277,9 +308,14 @@ Theorem wp_invariance {T} OpT Σ Λ `{invPreG Σ} s (e: proc OpT T) σ1 t2 σ2 �
 Proof.
   intros Hwp Hpartial.
   apply bind_star_inv_rep_n in Hpartial as (n&Hpartial).
-  eapply (soundness (M:=iResUR Σ) _ (S (S n))).
+  eapply (soundness (M:=iResUR Σ) _ (S k + S (S n))).
+  rewrite laterN_plus.
+  iApply bupd_iter_laterN_mono; first by reflexivity.
   iMod wsat_alloc as (Hinv) "[Hw HE]". specialize (Hwp _).
-  rewrite {1}uPred_fupd_eq in Hwp; iMod (Hwp with "[$Hw $HE]") as ">(Hw & HE & Hwp)".
+  iModIntro. iNext.
+  iApply (bupd_iter_mono k with "[Hw HE] []"); last by iApply Hwp.
+  iIntros "Hwp". rewrite {1}uPred_fupd_eq.
+  iMod ("Hwp" with "[$Hw $HE]") as ">(Hw & HE & Hwp)".
   iDestruct "Hwp" as (Istate) "(HIstate & Hwp & Hclose)".
   iApply (@wptp_invariance _ _ _ (IrisG _ _ _ Hinv Istate)); eauto with iFrame.
 Qed.
@@ -294,7 +330,7 @@ Corollary wp_invariance' {T} OpT Σ Λ `{invPreG Σ} s (e: proc OpT T) σ1 t2 σ
   Λ.(exec_partial) e σ1 (Val σ2 t2) →
   φ.
 Proof.
-  intros Hwp. eapply wp_invariance; first done.
+  intros Hwp. eapply wp_invariance with (k := O); first done.
   intros Hinv. iMod (Hwp Hinv) as (stateI) "(? & ? & Hφ)".
   iModIntro. iExists stateI. iFrame. iIntros "Hσ".
   iDestruct ("Hφ" with "Hσ") as (E) ">Hφ".
@@ -303,269 +339,77 @@ Qed.
 
 Import RelationNotations.
 
-Theorem wp_recovery_nonstuck {T R} OpT Σ Λ `{invPreG Σ} s (e: proc OpT T) (rec: proc OpT R)
-        σ1 φ φinv (φrec : Λ.(State) → Prop) :
-  (* normal execution *)
-  (∀ `{Hinv : invG Σ},
-     (|={⊤}=> ∃ stateI : State Λ → iProp Σ,
-       let _ : irisG OpT Λ Σ := IrisG _ _ _ Hinv stateI in
-       stateI σ1 ∗ WP e @ s; ⊤ {{ v, ∀ σ, stateI σ ={⊤,∅}=∗ ⌜φ v σ⌝ }}
-         ∗ (∀ σ2', stateI σ2' ={⊤,∅}=∗ ⌜φinv σ2'⌝))%I) →
-  (* recovery *)
-  (∀ `{Hinv : invG Σ} σ1 σ1' (Hφinv: φinv σ1) (Hcrash: Λ.(crash_step) σ1 (Val σ1' tt)),
-     (|={⊤}=> ∃ stateI : State Λ → iProp Σ,
-       let _ : irisG OpT Λ Σ := IrisG _ _ _ Hinv stateI in
-       stateI σ1' ∗ WP rec @ s; ⊤ {{ _, ∀ σ, stateI σ ={⊤, ∅}=∗ ⌜φrec σ⌝ }}
-         ∗ (∀ σ2', stateI σ2' ={⊤,∅}=∗ ⌜φinv σ2'⌝))%I) →
-    s = NotStuck →
-    ¬ Λ.(rexec) e (rec_singleton rec) σ1 Err.
+Lemma exec_rec_iter_split {R} OpT (Λ: Layer OpT) (rec: proc OpT R) σhalt ret:
+  (_ <- seq_star (_ <- Λ.(crash_step); exec_halt Λ rec); _ <- Λ.(crash_step); exec_halt Λ rec)
+    σhalt ret →
+  ∃ σcrash σrec : Λ.(State),
+    seq_star (_ <- Λ.(crash_step); exec_halt Λ rec) σhalt (Val σcrash ())
+    ∧ Λ.(crash_step) σcrash (Val σrec ())
+    ∧ exec_halt Λ rec σrec ret.
 Proof.
-  - rewrite /rexec/exec_recover => Hwp_e Hwp_rec Hnstuck Hrexec.
-    eapply rimpl_elim in Hrexec; last first.
-    { setoid_rewrite exec_seq_partial_singleton.
-      setoid_rewrite <-bind_assoc at 2.
-      setoid_rewrite seq_unit_sliding.
-      setoid_rewrite bind_assoc.
-      reflexivity.
-    }
-    assert (Hrexec' : (_ <- exec_partial Λ e; _ <- seq_star (_ <- Λ.(crash_step); exec_halt Λ rec);
-            _ <- Λ.(crash_step); exec_seq Λ (rec_singleton rec)) σ1 Err).
-    { intuition. }
-    clear Hrexec.
-    (* Show that φ is preserved after halt of e *)
-    destruct Hrexec' as [|(tp&σhalt&Hpartial&Hrec)].
-    { eapply wp_strong_adequacy; eauto.
-      intros Hinv.
-      iMod Hwp_e as (stateI) "[Hσ [H Hφ]]". iExists stateI. iIntros "{$Hσ} {$H} !> "; auto.
-    }
-    assert (Hφ: φinv σhalt).
-    { eapply wp_invariance; eauto.
-      intros Hinv.
-      iMod Hwp_e as (stateI) "[Hσ [H Hφ]]". iExists stateI. iIntros "{$Hσ} !>".
-      iSplitL "H"; last by iApply "Hφ".
-      iApply (wp_mono with "H"); eauto.
-    }
-    clear Hpartial Hwp_e.
+  intros Hrec. destruct ret as [b t|].
+  {
+    destruct Hrec as ([]&σhalt_rec&Hhd&([]&?&?&?)).
+    do 2 eexists; split_and!; eauto.
+  }
+  {
     destruct Hrec as [Hstar_err|([]&σhalt_rec&Hhd&Hrest)].
-    { remember Err as ret eqn:Heq.
+    - remember Err as ret eqn:Heq.
       revert Heq; induction Hstar_err; intros; try congruence; subst.
-      * apply IHHstar_err; auto.
-        destruct H0 as ([]&σ1'&?&?).
-        destruct H1 as (?&?&?&Hpure). inversion Hpure; subst.
-        eapply wp_invariance; eauto.
-        intros Hinv.
-        iMod Hwp_rec as (stateI) "[Hσ [H Hφ]]"; eauto. iExists stateI. iIntros "{$Hσ} !>".
-        iSplitL "H"; last by iApply "Hφ".
-        iApply (wp_mono with "H"); eauto.
-      * destruct H0 as [|([]&σ1'&?&?)].
-        { eapply crash_non_err; eauto. }
-        eapply bind_pure_no_err in H1.
-        eapply wp_adequacy with (φ0 := λ _, True); eauto.
-        intros Hinv.
-        iMod Hwp_rec as (stateI) "[Hσ [H Hφ]]"; eauto. iExists stateI. iIntros "{$Hσ} !>".
-        iApply (wp_mono with "H"); eauto.
-    }
-    (* Show that φ is preserved after crash + halt of rec *)
-    assert (Hφhalt_rec: φinv σhalt_rec).
-    {
-      clear Hrest.
-      remember (Val σhalt_rec ()) as ret eqn: Heq.
-      revert σhalt_rec Heq.
-      induction Hhd as [? []| x y z [] Hhd Hstar IH|]; inversion 1; subst; eauto.
-      eapply IH; eauto.
-      clear IH Hstar.
-      destruct Hhd as ([]&σcrash&Hcrash&Hhalt).
-      inversion Hhalt as (tp'&?&Hpartial&Hpure); subst.
-      inversion Hpure; subst.
-      eapply wp_invariance; eauto.
-      intros Hinv.
-      iMod Hwp_rec as (stateI) "[Hσ [H Hφ]]"; eauto. iExists stateI. iIntros "{$Hσ} !>".
-      iSplitL "H"; last by iApply "Hφ".
-      iApply (wp_mono with "H"); eauto.
-    }
-    clear Hhd Hφ.
-    destruct Hrest as [Hhd|Hrest].
-    { eapply crash_non_err; eauto. }
-    destruct Hrest as ([]&σcrash&Hcrash&[Hexec|(?&?&?&Hfalse)]); last first.
-    { inversion Hfalse. }
-    destruct Hexec as [|(l&?&?&Hmatch)]; last first.
-    { destruct l as [|(?&[])]; inversion Hmatch. }
-    edestruct (wp_strong_adequacy _ s rec σcrash (λ _ σ2, φrec σ2)) as (Had&?); eauto; last first.
-    { intuition eauto. }
-    intros Hinv.
-    iMod Hwp_rec as (stateI) "[Hσ [H Hφ]]"; eauto.
-    iExists stateI. iIntros "{$Hσ} {$H} !> "; auto.
+      * edestruct IHHstar_err as (σcrash&σrec_err&Hstar&?); auto.
+        exists σcrash, σrec_err; split; auto.
+        econstructor; eauto.
+      * destruct H as [|([]&σ&?&?)].
+        { exfalso. eapply crash_non_err; eauto. }
+        exists x, σ; split; auto.
+        econstructor.
+    - destruct Hrest as [|([]&σ&?&?)].
+      { exfalso. eapply crash_non_err; eauto. }
+      do 2 eexists; split_and!; eauto.
+  }
 Qed.
 
-Theorem wp_recovery_adequacy {T R} OpT Σ Λ `{invPreG Σ} s (e: proc OpT T) (rec: proc OpT R)
-        σ1 φ φinv (φrec : Λ.(State) → Prop) :
-  (* normal execution *)
-  (∀ `{Hinv : invG Σ},
-     (|={⊤}=> ∃ stateI : State Λ → iProp Σ,
-       let _ : irisG OpT Λ Σ := IrisG _ _ _ Hinv stateI in
-       stateI σ1 ∗ WP e @ s; ⊤ {{ v, ∀ σ, stateI σ ={⊤,∅}=∗ ⌜φ v σ⌝ }}
-         ∗ (∀ σ2', stateI σ2' ={⊤,∅}=∗ ⌜φinv σ2'⌝))%I) →
-  (* recovery *)
-  (∀ `{Hinv : invG Σ} σ1 σ1' (Hφinv: φinv σ1) (Hcrash: Λ.(crash_step) σ1 (Val σ1' tt)),
-     (|={⊤}=> ∃ stateI : State Λ → iProp Σ,
-       let _ : irisG OpT Λ Σ := IrisG _ _ _ Hinv stateI in
-       stateI σ1' ∗ WP rec @ s; ⊤ {{ _, ∀ σ, stateI σ ={⊤, ∅}=∗ ⌜φrec σ⌝ }}
-         ∗ (∀ σ2', stateI σ2' ={⊤,∅}=∗ ⌜φinv σ2'⌝))%I) →
-  s = NotStuck →
-  recv_adequate s e rec σ1 φ φrec.
-Proof.
-  intros Hwp_e Hwp_rec. split.
-  - intros σ2 ? Hexec. eapply wp_strong_adequacy; eauto.
-    intros Hinv.
-    iMod Hwp_e as (stateI) "[Hσ [H Hφ]]". iExists stateI. iIntros "{$Hσ} {$H} !> "; auto.
-  - rewrite /rexec/exec_recover => σ2 [] Hrexec.
-    eapply requiv_no_err_elim in Hrexec; first last.
-    { eapply wp_recovery_nonstuck; eauto. }
-    { setoid_rewrite exec_seq_partial_singleton.
-      setoid_rewrite <-bind_assoc at 2.
-      setoid_rewrite <-seq_unit_sliding_equiv.
-      setoid_rewrite bind_assoc.
-      reflexivity.
-    }
-    destruct Hrexec as (tp&σhalt&Hpartial&Hrec).
-    (* Show that φ is preserved after halt of e *)
-    assert (Hφ: φinv σhalt).
-    { eapply wp_invariance; eauto.
-      intros Hinv.
-      iMod Hwp_e as (stateI) "[Hσ [H Hφ]]". iExists stateI. iIntros "{$Hσ} !>". (*  *)
-      iSplitL "H"; last by iApply "Hφ".
-      iApply (wp_mono with "H"); eauto.
-    }
-    clear Hpartial Hwp_e.
-    destruct Hrec as ([]&σhalt_rec&Hhd&Hrest).
-    (* Show that φ is preserved after crash + halt of rec *)
-    assert (Hφhalt_rec: φinv σhalt_rec).
-    {
-      clear Hrest.
-      remember (Val σhalt_rec ()) as ret eqn: Heq.
-      revert σhalt_rec Heq.
-      induction Hhd as [? []| x y z [] Hhd Hstar IH|]; inversion 1; subst; eauto.
-      eapply IH; eauto.
-      clear IH Hstar.
-      destruct Hhd as ([]&σcrash&Hcrash&Hhalt).
-      inversion Hhalt as (tp'&?&Hpartial&Hpure); subst.
-      inversion Hpure; subst.
-      eapply wp_invariance; eauto.
-      intros Hinv.
-      iMod Hwp_rec as (stateI) "[Hσ [H Hφ]]"; eauto. iExists stateI. iIntros "{$Hσ} !>".
-      iSplitL "H"; last by iApply "Hφ".
-      iApply (wp_mono with "H"); eauto.
-    }
-    clear Hhd Hφ.
-    destruct Hrest as ([]&σcrash&Hcrash&(tp'&?&Hexec&Hp)); subst.
-    inversion Hp; subst.
-    edestruct (wp_strong_adequacy _ NotStuck
-                                  rec σcrash (λ _ σ2, φrec σ2)) as (Had&?); eauto; last first.
-    { edestruct Had; intuition eauto. }
-    intros Hinv.
-    iMod Hwp_rec as (stateI) "[Hσ [H Hφ]]"; eauto.
-    iExists stateI. iIntros "{$Hσ} {$H} !> "; auto.
-  - eapply wp_recovery_nonstuck; eauto.
-Qed.
+Inductive seq_star_exec_steps {R} {OpT} {Λ: Layer OpT} (rec: proc OpT R)
+  : Λ.(State) → Λ.(State) → nat → Prop :=
+  | sses_nil σ :
+      seq_star_exec_steps rec σ σ O
+  | sses_cons σ1 σ1' σ2 ret σ3 k n :
+      Λ.(crash_step) σ1 (Val σ1' ()) →
+      bind_rep_n n (exec_pool Λ) [existT R rec] σ1' (Val σ2 ret) →
+      seq_star_exec_steps rec σ2 σ3 k →
+      seq_star_exec_steps rec σ1 σ3 (S n + S k).
 
-Theorem wp_recovery_invariance {T R} OpT Σ Λ `{invPreG Σ} s (e: proc OpT T) (rec: proc OpT R)
-        σ1 (φinv ρ : Λ.(State) → Prop) :
-  (* φ is an invariant of normal execution *)
-  (∀ `{Hinv : invG Σ},
-     (|={⊤}=> ∃ stateI : State Λ → iProp Σ,
-       let _ : irisG OpT Λ Σ := IrisG _ _ _ Hinv stateI in
-       stateI σ1 ∗ WP e @ s; ⊤ {{ _, True }} ∗ (∀ σ2', stateI σ2' ={⊤,∅}=∗ ⌜φinv σ2'⌝))%I) →
-  (* φ is an invariant of recovery execution *)
-  (∀ `{Hinv : invG Σ} σ1 σ1' (Hφ: φinv σ1) (Hcrash: Λ.(crash_step) σ1 (Val σ1' tt)),
-     (|={⊤}=> ∃ stateI : State Λ → iProp Σ,
-       let _ : irisG OpT Λ Σ := IrisG _ _ _ Hinv stateI in
-       stateI σ1' ∗ WP rec @ s; ⊤ {{ _, True }} ∗ (∀ σ2', stateI σ2' ={⊤,∅}=∗ ⌜φinv σ2'⌝))%I) →
-  (∀ σ, φinv σ → ρ σ) →
-  (∀ σ1 σ2, φinv σ1 → Λ.(crash_step) σ1 (Val σ2 tt) → ρ σ2) →
-  s = NotStuck →
-  (∀ σ2 t2, Λ.(rexec_partial) e (rec_singleton rec) σ1 (Val σ2 t2) → ρ σ2)
-    ∧ recv_adequate s e rec σ1 (fun _ _ => True) (fun _ => True).
+Lemma seq_star_exec_steps_intro {R} {OpT} {Λ: Layer OpT} (rec: proc OpT R) σhalt σcrash:
+  seq_star (_ <- Λ.(crash_step); exec_halt Λ rec) σhalt (Val σcrash ()) →
+  ∃ k, seq_star_exec_steps rec σhalt σcrash k.
 Proof.
-  intros Hwp_e Hwp_rec Himpl Hcrash_impl Hnonstuck.
-  assert (recv_adequate s e rec σ1 (fun _ _ => True) (fun _ => True)).
-  {
-    eapply wp_recovery_adequacy; first eauto.
-    - intros. iMod Hwp_e as (stateI) "[Hσ [H Hφ]]"; eauto. iExists stateI.
-      iIntros "{$Hσ} {$Hφ} !>".
-      iApply (wp_mono with "H"); eauto.
-      iIntros. iApply fupd_mask_weaken; auto.
-    - intros. iMod Hwp_rec as (stateI) "[Hσ [H Hφ]]"; eauto. iExists stateI.
-      iIntros "{$Hσ} !>".
-      iSplitL "H"; last eauto.
-      iApply (wp_mono with "H"); eauto.
-      iIntros. iApply fupd_mask_weaken; auto.
-    - eauto.
-  }
-  split; auto.
-  intros σ2 t2 Hpartial.
-  unfold rexec_partial, exec_recover_partial in Hpartial.
-  eapply requiv_no_err_elim in Hpartial; first last.
-  { intros Herr. apply rexec_partial_err_rexec_err in Herr.
-    eapply recv_adequate_not_stuck; eauto.
-  }
-  { setoid_rewrite exec_seq_partial_singleton.
-    setoid_rewrite <-bind_assoc at 2.
-    setoid_rewrite <-bind_assoc at 2.
-    setoid_rewrite <-seq_unit_sliding_equiv.
-    setoid_rewrite bind_assoc.
-    setoid_rewrite bind_assoc.
-    reflexivity.
-  }
-  destruct Hpartial as (tp&σhalt&Hpartial&Hrec).
-  (* Show that φ is preserved after halt of e *)
-  assert (Hφ: φinv σhalt).
-  { eapply wp_invariance; eauto.
-    intros Hinv.
-    iMod Hwp_e as (stateI) "[Hσ [H Hφ]]". iExists stateI. iIntros "{$Hσ} {$H} !> Hσ".
-      by iApply "Hφ".
-  }
-  clear Hpartial Hwp_e.
-  destruct Hrec as ([]&σhalt_rec&Hhd&Hrest).
-  (* Show that φ is preserved after crash + halt of rec *)
-  assert (Hφ_halt: ∀ σhalt σhalt_rec,
-             φinv σhalt ->
-             (_ <- Λ.(crash_step); exec_halt Λ rec) σhalt (Val σhalt_rec ()) ->
-             φinv σhalt_rec).
-  {
-    intros ??? ([]&σcrash&Hcrash&Hhalt).
-    destruct Hhalt as (tp'&?&Hpartial&Hp); subst.
-    inversion Hp; subst.
-    eapply wp_invariance; eauto.
-    intros Hinv.
-    iMod Hwp_rec as (stateI) "[Hσ [H Hφ]]"; eauto. iExists stateI. iIntros "{$Hσ} {$H} !> Hσ".
-      by iApply "Hφ".
-  }
-  cut (φinv σhalt_rec).
-  destruct t2. intros Hrec.
-  eapply Himpl, Hφ_halt; eauto.
-  clear Hwp_rec. clear Hrest.
-  remember (Val σhalt_rec ()) as ret eqn:Heq.
-  revert σhalt_rec Heq. induction Hhd; eauto.
-  - intros. inversion Heq; subst. eauto.
-  - intros; subst. eapply IHHhd; eauto.
-    eapply Hφ_halt; eauto. destruct o1; eauto.
-  - congruence.
+  intros Hstar.
+  remember (Val σcrash ()) as ret eqn:Heq; revert Heq.
+  induction Hstar as [|??? [] Hstep|]; inversion 1; subst.
+  - exists O. econstructor.
+  - destruct Hstep as ([]&σ'&Hcrash&Hexec).
+    edestruct IHHstar as (k&Hrest); auto.
+    destruct Hexec as (?&?&Hpartial&Hpure).
+    inversion Hpure; subst.
+    apply bind_star_inv_rep_n in Hpartial as (n&Hbind).
+    exists (S n + S k)%nat; econstructor; eauto.
 Qed.
 
 Theorem wp_recovery_nonstuck_internal {T R} OpT Σ Λ `{invPreG Σ} s (e: proc OpT T) (rec: proc OpT R)
-        σ1 φ φinv (φrec : Λ.(State) → iProp Σ) :
-  (* normal execution *)
+        σ1 φ φinv φrec :
   (∀ `{Hinv : invG Σ},
+     (* normal execution *)
      (|={⊤}=> ∃ stateI : State Λ → iProp Σ,
        let _ : irisG OpT Λ Σ := IrisG _ _ _ Hinv stateI in
-       stateI σ1 ∗ WP e @ s; ⊤ {{ v, ∀ σ, stateI σ ={⊤,∅}=∗ ⌜φ v σ⌝ }}
-       ∗ (∀ σ2', stateI σ2' ={⊤,∅}=∗ φinv σ2'))
+       stateI σ1 ∗ WP e @ s; ⊤ {{ v, ∀ σ, stateI σ ={⊤,∅}=∗ ⌜ φ v σ ⌝ }}
+       ∗ (∀ σ2', stateI σ2' ={⊤,∅}=∗ φinv σ2')
      ∗
-     (∀ `{Hinv : invG Σ} σ1 σ1' (Hcrash: Λ.(crash_step) σ1 (Val σ1' tt)),
+     (* recovery execution *)
+     □ (∀ `{Hinv : invG Σ} σ1 σ1' (Hcrash: Λ.(crash_step) σ1 (Val σ1' tt)),
      (φinv σ1 ={⊤}=∗ ∃ stateI : State Λ → iProp Σ,
        let _ : irisG OpT Λ Σ := IrisG _ _ _ Hinv stateI in
-       stateI σ1' ∗ WP rec @ s; ⊤ {{ _, ∀ σ, stateI σ ={⊤, ∅}=∗ φrec σ }}
-         ∗ (∀ σ2', stateI σ2' ={⊤,∅}=∗ φinv σ2'))))%I →
+       stateI σ1' ∗ WP rec @ s; ⊤ {{ _, ∀ σ, stateI σ ={⊤, ∅}=∗ ⌜ φrec σ ⌝ }}
+         ∗ (∀ σ2', stateI σ2' ={⊤,∅}=∗ φinv σ2')))))%I →
     s = NotStuck →
     ¬ Λ.(rexec) e (rec_singleton rec) σ1 Err.
 Proof.
@@ -575,7 +419,7 @@ Proof.
       setoid_rewrite <-bind_assoc at 2.
       setoid_rewrite seq_unit_sliding.
       setoid_rewrite bind_assoc.
-      simpl exec_seq. SearchAbout exec.
+      simpl exec_seq.
       setoid_rewrite exec_halt_finish.
       reflexivity.
     }
@@ -585,81 +429,298 @@ Proof.
     clear Hrexec.
     (* Show that we couldn't have crashed during e *)
     destruct Hrexec' as [|(tp&σhalt&Hpartial&Hrec)].
-    { eapply wp_strong_adequacy; eauto.
+    { eapply wp_strong_adequacy with (k := O); eauto.
       intros Hinv.
-      iDestruct (Hwp $! _) as "(Hwp_e&Hwp_rec)".
-      iMod "Hwp_e" as (stateI) "[Hσ [H Hφ]]". iExists stateI. iIntros "{$Hσ} {$H} !> "; auto.
-    }
-    assert (∃ σcrash σrec_err,
-               (seq_star (_ <- Λ.(crash_step); exec_halt Λ rec) σhalt (Val σcrash tt) ∧
-                Λ.(crash_step) σcrash (Val σrec_err tt) ∧
-                exec_halt Λ rec σrec_err Err))
-     as (σcrash&σrec_err&Hstar&Hcrash&Herr).
-    {
-      clear -Hrec.
-      destruct Hrec as [Hstar_err|([]&σhalt_rec&Hhd&Hrest)].
-      - remember Err as ret eqn:Heq.
-        revert Heq; induction Hstar_err; intros; try congruence; subst.
-        * edestruct IHHstar_err as (σcrash&σrec_err&Hstar&?); auto.
-          exists σcrash, σrec_err; split; auto.
-          econstructor; eauto.
-        * destruct H as [|([]&σ&?&?)].
-          { exfalso. eapply crash_non_err; eauto. }
-          exists x, σ; split; auto.
-          econstructor.
-      - destruct Hrest as [|([]&σ&?&?)].
-          { exfalso. eapply crash_non_err; eauto. }
-          do 2 eexists; split_and!; eauto.
+      iPoseProof (Hwp $! Hinv) as "Hwp".
+      iMod "Hwp" as (stateI) "(Hσ&Hwp_e&?&_)".
+      iExists stateI. iIntros "{$Hσ} !> "; auto.
     }
 
-    edestruct (wp_strong_adequacy _ s rec σrec_err (λ _ σ2, True)) as (Had&?); eauto; last first.
-    { apply bind_pure_no_err in Herr; intuition. }
+    edestruct (@exec_rec_iter_split)
+        as (σcrash&σrec_err&Hstar&Hcrash&Herr); eauto.
+
+    apply bind_star_inv_rep_n in Hpartial as (n&Hpartial).
+    apply seq_star_exec_steps_intro in Hstar as (k&Hstar).
+    apply bind_pure_no_err in Herr.
+    edestruct (bind_star_inv_rep_n) as (n'&Herr'); first by eapply Herr.
+
+    edestruct (wp_strong_adequacy _ s rec σrec_err (λ _ σ2, True)
+               (S n + S k )) as (Had&?); eauto; last first.
+    { intuition. }
+
 
     intros Hinv.
+    rewrite Nat_iter_add.
     iMod wsat_alloc as (Hinv') "[Hw HE]".
-    iPoseProof (Hwp $! Hinv') as "(Hwp_e&Hwp_rec)".
-    iAssert (|==> ◇ φinv σhalt)%I with "[Hw HE]" as ">>Hσhalt".
+    iPoseProof (Hwp $! Hinv') as "Hwp".
+    rewrite uPred_fupd_eq.
+    iMod ("Hwp" with "[$Hw $HE]") as ">(Hw & HE & Hrest)".
+    iDestruct "Hrest" as (stateI) "(Hσ&Hwp_e&Hinv&#Hwp_rec)".
+    iAssert (Nat.iter (S n) (λ P, |==> ▷ P)%I (|==> ◇ φinv σhalt))%I with "[Hw HE Hσ Hwp_e Hinv]"
+      as "Hσhalt".
     {
-      iClear "Hwp_rec".
-      rewrite uPred_fupd_eq.
-      iMod ("Hwp_e" with "[$Hw $HE]") as ">(Hw & HE & Hrest)".
-      iDestruct "Hrest" as (stateI) "(Hs&Hwp&Hinv)".
-      iSpecialize ("Hinv" $! σhalt with "[Hs Hwp]").
-      (* need to show you can obtain state interp for anything you can reduce to
-         from initial and weakest pre*)
-      { admit. }
-      rewrite /uPred_fupd_def.
-      iMod ("Hinv" with "[$Hw $HE]") as ">(?&?&$)".
-      done.
+      iDestruct (wptp_steps_state_inv with "[-Hinv]") as "H".
+      { eapply Hpartial. }
+      { iFrame. done. }
+      iApply (bupd_iter_mono with "[Hinv] H").
+      iIntros "(Hw&HE&Hstate)". iSpecialize ("Hinv" with "Hstate").
+      iMod ("Hinv" with "[$Hw $HE]") as "(?&?&$)"; auto.
     }
-    clear Hpartial Hrec.
-    iClear "Hwp_e".
+    iApply (bupd_iter_mono with "[] Hσhalt"); iIntros "Hσhalt".
 
-    iAssert (|==> ◇ φinv σcrash)%I with "[Hσhalt]" as ">>Hinv'".
+    iClear "Hwp".
+    clear Hpartial Hrec.
+
+    iAssert (Nat.iter (S k) (λ P, |==> ▷ P)%I (|==> ◇ φinv σcrash))%I with "[Hσhalt]" as "Hinv'".
     {
-      clear Hcrash σrec_err Herr.
-      remember (Val σcrash ()) as ret eqn:Heq.
-      iInduction Hstar as [?|x y ? ? Hstep Hstar|?] "IH" forall (Heq); inversion Heq; subst; auto.
+      clear Hcrash σrec_err Herr Herr'.
+      iInduction Hstar as [| σhalt σhalt' σmid ret σcrash k m Hcrash Hrep Hind ] "IH".
+      { iIntros "!> !>"; auto. }
+
+      rewrite (Nat_iter_S (S m + S k)).
+      rewrite Nat_iter_add.
+      iMod wsat_alloc as (Hinv'') "[Hw HE]".
+      iSpecialize ("Hwp_rec" $! _ _ _ Hcrash).
+      rewrite uPred_fupd_eq.
+      iMod "Hσhalt". iModIntro. iMod "Hσhalt". iNext.
+      iMod ("Hwp_rec" with "Hσhalt [$Hw $HE]") as ">(Hw & HE & Hrest)".
+      iDestruct "Hrest" as (stateI') "(Hs&Hwp&Hinv)".
+      iDestruct (wptp_steps_state_inv with "[-Hinv]") as "H".
+      { eapply Hrep. }
+      { iFrame. done. }
+      iApply (bupd_iter_mono with "[Hinv] H").
+      iIntros "(Hw&HE&Hstate)".
+      iApply "IH"; auto.
+      iSpecialize ("Hinv" with "[Hstate]"); eauto.
+      rewrite /uPred_fupd_def.
+      by iMod ("Hinv" with "[$Hw $HE]") as ">(?&?&$)".
+    }
+
+
+    iApply (bupd_iter_mono with "[] Hinv'"); iIntros ">>Hinv'".
+    iSpecialize ("Hwp_rec" $! Hinv σcrash σrec_err Hcrash with "Hinv'").
+    iMod "Hwp_rec" as (stateI'') "[Hσ [H _]]"; eauto.
+    iExists stateI''. iIntros "{$Hσ} !> "; auto.
+    iApply wp_wand_l; iFrame.
+    iIntros (?) "Hwand". iIntros. iApply @fupd_mask_weaken; auto.
+Qed.
+
+Theorem wp_recovery_adequacy {T R} OpT Σ Λ `{invPreG Σ} s (e: proc OpT T) (rec: proc OpT R)
+        σ1 φ φinv (φrec : Λ.(State) → Prop) :
+  (∀ `{Hinv : invG Σ},
+     (* normal execution *)
+     (|={⊤}=> ∃ stateI : State Λ → iProp Σ,
+       let _ : irisG OpT Λ Σ := IrisG _ _ _ Hinv stateI in
+       stateI σ1 ∗ WP e @ s; ⊤ {{ v, ∀ σ, stateI σ ={⊤,∅}=∗ ⌜ φ v σ ⌝ }}
+       ∗ (∀ σ2', stateI σ2' ={⊤,∅}=∗ φinv σ2')
+     ∗
+     (* recovery execution *)
+     □ (∀ `{Hinv : invG Σ} σ1 σ1' (Hcrash: Λ.(crash_step) σ1 (Val σ1' tt)),
+     (φinv σ1 ={⊤}=∗ ∃ stateI : State Λ → iProp Σ,
+       let _ : irisG OpT Λ Σ := IrisG _ _ _ Hinv stateI in
+       stateI σ1' ∗ WP rec @ s; ⊤ {{ _, ∀ σ, stateI σ ={⊤, ∅}=∗ ⌜ φrec σ ⌝ }}
+         ∗ (∀ σ2', stateI σ2' ={⊤,∅}=∗ φinv σ2')))))%I →
+  s = NotStuck →
+  recv_adequate s e rec σ1 φ φrec.
+Proof.
+  intros Hwp ?. split.
+  - intros σ2 ? Hexec. eapply wp_strong_adequacy with (k := 0); eauto.
+    intros Hinv.
+    iPoseProof (Hwp $! Hinv) as "Hwp".
+    iMod "Hwp" as (stateI) "(Hσ&Hwp_e&?&_)".
+    iExists stateI. iIntros "{$Hσ} !> "; auto.
+  - rewrite /rexec/exec_recover => σ2 [] Hrexec.
+    eapply requiv_no_err_elim in Hrexec; first last.
+    { eapply wp_recovery_nonstuck_internal; eauto. }
+    { setoid_rewrite exec_seq_partial_singleton.
+      setoid_rewrite <-bind_assoc at 2.
+      setoid_rewrite <-seq_unit_sliding_equiv.
+      setoid_rewrite bind_assoc.
+      reflexivity.
+    }
+    simpl exec_seq in Hrexec.
+
+    destruct Hrexec as (tp&σhalt&Hpartial&Hrec).
+    destruct Hrec as ([]&σcrash&Hstar&Hfin).
+    destruct Hfin as ([]&σcrash'&Hcrash&Hfin).
+
+
+    apply bind_star_inv_rep_n in Hpartial as (n&Hpartial).
+    apply seq_star_exec_steps_intro in Hstar as (k&Hstar).
+    destruct Hfin as (?&?&Hexec&Hp).
+    inversion Hp; subst. clear Hp.
+
+    edestruct (wp_strong_adequacy _ NotStuck rec σcrash' (λ _ s, φrec s)
+               (S n + S k )) as (Had&?); eauto; last first.
+    { edestruct Had; intuition eauto. }
+
+
+    intros Hinv.
+    rewrite Nat_iter_add.
+    iMod wsat_alloc as (Hinv') "[Hw HE]".
+    iPoseProof (Hwp $! Hinv') as "Hwp".
+    rewrite uPred_fupd_eq.
+    iMod ("Hwp" with "[$Hw $HE]") as ">(Hw & HE & Hrest)".
+    iDestruct "Hrest" as (stateI) "(Hσ&Hwp_e&Hinv&#Hwp_rec)".
+    iAssert (Nat.iter (S n) (λ P, |==> ▷ P)%I (|==> ◇ φinv σhalt))%I with "[Hw HE Hσ Hwp_e Hinv]"
+      as "Hσhalt".
+    {
+      iDestruct (wptp_steps_state_inv with "[-Hinv]") as "H".
+      { eapply Hpartial. }
+      { iFrame. done. }
+      iApply (bupd_iter_mono with "[Hinv] H").
+      iIntros "(Hw&HE&Hstate)". iSpecialize ("Hinv" with "Hstate").
+      iMod ("Hinv" with "[$Hw $HE]") as "(?&?&$)"; auto.
+    }
+    iApply (bupd_iter_mono with "[] Hσhalt"); iIntros "Hσhalt".
+
+    iClear "Hwp".
+    clear Hpartial.
+
+    iAssert (Nat.iter (S k) (λ P, |==> ▷ P)%I (|==> ◇ φinv σcrash))%I with "[Hσhalt]" as "Hinv'".
+    {
+      clear Hcrash Hexec σcrash' σ2 x Hexec.
+      iInduction Hstar as [| σhalt σhalt' σmid ret σcrash k m Hcrash Hrep Hind ] "IH".
+      { iIntros "!> !>"; auto. }
+
+      rewrite (Nat_iter_S (S m + S k)).
+      rewrite Nat_iter_add.
       iMod wsat_alloc as (Hinv'') "[Hw HE]".
       iSpecialize ("Hwp_rec" $! Hinv'').
-      destruct Hstep as ([]&σrec_err&Hcrash&?).
-      iSpecialize ("Hwp_rec" $! _ σrec_err Hcrash).
+      iSpecialize ("Hwp_rec" $! _ _ Hcrash).
       rewrite uPred_fupd_eq.
+      iMod "Hσhalt". iModIntro. iMod "Hσhalt". iNext.
       iMod ("Hwp_rec" with "Hσhalt [$Hw $HE]") as ">(Hw & HE & Hrest)".
-      iDestruct "Hrest" as (stateI) "(Hs&Hwp&Hinv)".
-      iSpecialize ("Hinv" $! y with "[Hs Hwp]").
-      (* need to show you can obtain state interp for anything you can reduce to
-         from initial and weakest pre*)
-      { admit. }
-      rewrite /uPred_fupd_def.
-      iMod ("Hinv" with "[$Hw $HE]") as ">(?&?&?)".
+      iDestruct "Hrest" as (stateI') "(Hs&Hwp&Hinv)".
+      iDestruct (wptp_steps_state_inv with "[-Hinv]") as "H".
+      { eapply Hrep. }
+      { iFrame. done. }
+      iApply (bupd_iter_mono with "[Hinv] H").
+      iIntros "(Hw&HE&Hstate)".
       iApply "IH"; auto.
+      iSpecialize ("Hinv" with "[Hstate]"); eauto.
+      rewrite /uPred_fupd_def.
+      by iMod ("Hinv" with "[$Hw $HE]") as ">(?&?&$)".
     }
 
 
-    iSpecialize ("Hwp_rec" $! Hinv σcrash σrec_err Hcrash with "Hinv'").
-    iMod "Hwp_rec" as (stateI) "[Hσ [H _]]"; eauto.
-    iExists stateI. iIntros "{$Hσ} !> "; auto.
-    iApply wp_wand_l; iFrame.
-    iIntros (?) "Hwand". iIntros (σ) "H". iMod ("Hwand" with "H"); auto.
-Admitted.
+    iApply (bupd_iter_mono with "[] Hinv'"); iIntros ">>Hinv'".
+    iSpecialize ("Hwp_rec" $! Hinv σcrash σcrash' Hcrash with "Hinv'").
+    iMod "Hwp_rec" as (stateI'') "[Hσ [H _]]"; eauto.
+    iExists stateI''. iIntros "{$Hσ} !> "; auto.
+  - eapply wp_recovery_nonstuck_internal; eauto.
+Qed.
+
+Theorem wp_recovery_invariance {T R} OpT Σ Λ `{invPreG Σ} s (e: proc OpT T) (rec: proc OpT R)
+        σ1 φ φrec φinv ρ :
+  (∀ `{Hinv : invG Σ},
+     (* normal execution *)
+     (|={⊤}=> ∃ stateI : State Λ → iProp Σ,
+       let _ : irisG OpT Λ Σ := IrisG _ _ _ Hinv stateI in
+       stateI σ1 ∗ WP e @ s; ⊤ {{ v, ∀ σ, stateI σ ={⊤,∅}=∗ ⌜ φ v σ ⌝ }}
+       ∗ (∀ σ2', stateI σ2' ={⊤,∅}=∗ φinv σ2' ∗ ⌜ ρ σ2' ⌝)
+     ∗
+     (* recovery execution *)
+     □ (∀ `{Hinv : invG Σ} σ1 σ1' (Hcrash: Λ.(crash_step) σ1 (Val σ1' tt)),
+     (φinv σ1 ={⊤}=∗ ∃ stateI : State Λ → iProp Σ,
+       let _ : irisG OpT Λ Σ := IrisG _ _ _ Hinv stateI in
+       stateI σ1' ∗ WP rec @ s; ⊤ {{ _, ∀ σ, stateI σ ={⊤, ∅}=∗ ⌜ φrec σ ⌝ }}
+         ∗ (∀ σ2', stateI σ2' ={⊤,∅}=∗ φinv σ2' ∗ ⌜ ρ σ2' ⌝)))))%I →
+  s = NotStuck →
+  (∀ σ2 t2, Λ.(rexec_partial) e (rec_singleton rec) σ1 (Val σ2 t2) → ρ σ2)
+    ∧ recv_adequate s e rec σ1 φ φrec.
+Proof.
+  intros Hwp ?.
+  assert (recv_adequate s e rec σ1 φ φrec).
+  {
+    eapply wp_recovery_adequacy with (φinv0 := φinv); first eauto.
+    - intros. iIntros. iPoseProof (Hwp $! Hinv) as "Hwp".
+      iMod "Hwp" as (stateI) "(Hσ&Hwp_e&Hφ&#Hwp_rec)".
+      iModIntro. iExists stateI. iFrame.
+      iSplitR "Hwp_rec".
+      * iIntros. iMod ("Hφ" with "[$]") as "($&?)"; auto.
+      * iIntros. iModIntro. iIntros.
+        iMod ("Hwp_rec" with "[//] [$]") as (stateI') "[Hσ [H Hφ]]"; eauto.
+        iExists stateI'.
+        iIntros "{$Hσ} {$H} !>". iIntros. iMod ("Hφ" with "[$]") as "($&?)"; auto.
+    - eauto.
+  }
+  split; auto. intros σ2 [] Hpartial.
+  unfold rexec_partial, exec_recover_partial in Hpartial.
+
+  eapply requiv_no_err_elim in Hpartial; first last.
+  { intros Herr. apply rexec_partial_err_rexec_err in Herr.
+    eapply recv_adequate_not_stuck; eauto. }
+  { setoid_rewrite exec_seq_partial_singleton.
+    setoid_rewrite <-bind_assoc at 2.
+    setoid_rewrite <-bind_assoc at 2.
+    setoid_rewrite <-seq_unit_sliding_equiv.
+    setoid_rewrite bind_assoc.
+    setoid_rewrite bind_assoc.
+    reflexivity.
+  }
+  destruct Hpartial as (tp&σhalt&Hpartial&Hrec).
+  destruct Hrec as ([]&σcrash&Hstar&([]&σrec&Hcrash&Hrec)).
+  destruct Hrec as (?&?&Hrec&Hpure). inversion Hpure; subst.
+  apply bind_star_inv_rep_n in Hpartial as (n&Hpartial).
+  apply seq_star_exec_steps_intro in Hstar as (k&Hstar).
+
+  eapply @wp_invariance with (k := (S n + S k)%nat); eauto.
+  intros Hinv.
+  rewrite Nat_iter_add.
+  iMod wsat_alloc as (Hinv') "[Hw HE]".
+  iPoseProof (Hwp $! Hinv') as "Hwp".
+  rewrite uPred_fupd_eq.
+  iMod ("Hwp" with "[$Hw $HE]") as ">(Hw & HE & Hrest)".
+  iDestruct "Hrest" as (stateI) "(Hσ&Hwp_e&Hinv&#Hwp_rec)".
+
+  iAssert (Nat.iter (S n) (λ P, |==> ▷ P)%I (|==> ◇ φinv σhalt))%I with "[Hw HE Hσ Hwp_e Hinv]"
+    as "Hσhalt".
+  {
+    iDestruct (wptp_steps_state_inv with "[-Hinv]") as "H".
+    { eapply Hpartial. }
+    { iFrame. done. }
+    iApply (bupd_iter_mono with "[Hinv] H").
+    iIntros "(Hw&HE&Hstate)". iSpecialize ("Hinv" with "Hstate").
+    iMod ("Hinv" with "[$Hw $HE]") as "(?&?&($&?))"; auto.
+  }
+  iApply (bupd_iter_mono with "[] Hσhalt"); iIntros "Hσhalt".
+
+  iClear "Hwp".
+  clear Hpartial.
+
+  iAssert (Nat.iter (S k) (λ P, |==> ▷ P)%I (|==> ◇ φinv σcrash))%I with "[Hσhalt]" as "Hinv'".
+  {
+    clear Hcrash Hrec σ2 Hpure.
+    iInduction Hstar as [| σhalt σhalt' σmid ret σcrash k m Hcrash Hrep Hind ] "IH".
+    { iIntros "!> !>"; auto. }
+
+    rewrite (Nat_iter_S (S m + S k)).
+    rewrite Nat_iter_add.
+    iMod wsat_alloc as (Hinv'') "[Hw HE]".
+    iSpecialize ("Hwp_rec" $! Hinv'').
+    iSpecialize ("Hwp_rec" $! _ _ Hcrash).
+    rewrite uPred_fupd_eq.
+    iMod "Hσhalt". iModIntro. iMod "Hσhalt". iNext.
+    iMod ("Hwp_rec" with "Hσhalt [$Hw $HE]") as ">(Hw & HE & Hrest)".
+    iDestruct "Hrest" as (stateI') "(Hs&Hwp&Hinv)".
+    iDestruct (wptp_steps_state_inv with "[-Hinv]") as "H".
+    { eapply Hrep. }
+    { iFrame. done. }
+    iApply (bupd_iter_mono with "[Hinv] H").
+    iIntros "(Hw&HE&Hstate)".
+    iApply "IH"; auto.
+    iSpecialize ("Hinv" with "[Hstate]"); eauto.
+    rewrite /uPred_fupd_def.
+    by iMod ("Hinv" with "[$Hw $HE]") as ">(?&?&($&?))".
+  }
+
+
+  iApply (bupd_iter_mono with "[] Hinv'"); iIntros ">>Hinv'".
+  iSpecialize ("Hwp_rec" $! Hinv σcrash _ Hcrash with "Hinv'").
+  iMod "Hwp_rec" as (stateI'') "[Hσ [H Hinv]]"; eauto.
+  iExists stateI''. iIntros "{$Hσ} !> "; auto.
+  iSplitL "H".
+  - iApply wp_wand_l; iFrame. iIntros; auto.
+  - iIntros. iMod ("Hinv" with "[$]") as "(?&$)"; auto.
+Qed.
