src/CSL/RefinementAdequacy.v
@@ -34,7 +34,7 @@ Require Import Helpers.RelationAlgebra.
 Theorem wp_recovery_crash_refinement {T R} OpTa OpTc Σ (Λa: Layer OpTa) (Λc: Layer OpTc)
         `{invPreG Σ} `{cfgPreG OpTa Λa Σ}
         (ea: proc OpTa T) (ec: proc OpTc T) (rec: proc OpTc R)
-        φ (absr: relation Λa.(State) Λc.(State) unit) E
+        φinv (absr: relation Λa.(State) Λc.(State) unit) E
         (Habsr_no_err: ∀ σa, ¬ absr σa Err):
   nclose sourceN ⊆ E →
   (∀ (σ1a: Λa.(State)) σ1c,
@@ -42,28 +42,26 @@ Theorem wp_recovery_crash_refinement {T R} OpTa OpTc Σ (Λa: Layer OpTa) (Λc: 
       (∀ `{Hinv : invG Σ} `{Hcfg: cfgG OpTa Λa Σ},
           (|={⊤}=> ∃ stateI : State Λc → iProp Σ,
              let _ : irisG OpTc Λc Σ := IrisG _ _ _ Hinv stateI in
-             (source_ctx ([existT _ ea], σ1a) ∗ O ⤇ ea ∗ source_state σ1a) -∗
-              stateI σ1c ∗ WP ec @ NotStuck; ⊤ {{ v, O ⤇ of_val v
+             (source_ctx ([existT _ ea], σ1a) ∗ O ⤇ ea ∗ source_state σ1a)
+               -∗
+               stateI σ1c
+               ∗ WP ec @ NotStuck; ⊤ {{ v, O ⤇ of_val v
                     ∗ (∀ σ2c, stateI σ2c ={⊤,E}=∗ ∃ σ2a, source_state σ2a ∗ ⌜absr σ2a (Val σ2c tt)⌝)}}
-                              ∗ (∀ σ2c, stateI σ2c ={⊤,E}=∗ ∃ tp σ2a, source_pool_map tp
-                                         ∗ source_state σ2a ∗ ⌜φ tp σ2a σ2c⌝))%I)) →
-  (∀ `{Hinv : invG Σ} `{Hcfg: cfgG OpTa Λa Σ}
-     tp1 tp1' σ1a σ1c σ1c'
-     (Hφ: φ tp1 σ1a σ1c)
-     (Htp_sub: pool_map_incl tp1 tp1')
-     (Hcrash: Λc.(crash_step) σ1c (Val σ1c' tt)),
-     (|={⊤}=> ∃ stateI : State Λc → iProp Σ,
-       let _ : irisG OpTc Λc Σ := IrisG _ _ _ Hinv stateI in
-       (source_ctx (tp1', σ1a) ∗ source_pool_map (tpool_to_map tp1') ∗ source_state σ1a) -∗
-              stateI σ1c' ∗ WP rec @ NotStuck; ⊤ {{ v, (∀ σ2c, stateI σ2c ={⊤,E}=∗
+                                     ∗ (∀ σ2c, stateI σ2c ={⊤,E}=∗ φinv σ2c)
+        ∗
+        □ (∀ `{Hinv : invG Σ} `{Hcfg: cfgG OpTa Λa Σ} σ1c σ1c'
+           (Hcrash: Λc.(crash_step) σ1c (Val σ1c' tt)),
+            (φinv σ1c ={⊤}=∗ ∃ stateI : State Λc → iProp Σ,
+               let _ : irisG OpTc Λc Σ := IrisG _ _ _ Hinv stateI in
+               stateI σ1c'
+               ∗ WP rec @ NotStuck; ⊤ {{ v, (∀ σ2c, stateI σ2c ={⊤,E}=∗
                    ∃ σ2a σ2a', source_state σ2a ∗ ⌜Λa.(crash_step) σ2a (Val σ2a' tt)
                                ∧ absr σ2a' (Val σ2c tt)⌝)}}
-                              ∗ (∀ σ2c, stateI σ2c ={⊤,E}=∗ ∃ tp σ2a, source_pool_map tp
-                                         ∗ source_state σ2a ∗ ⌜φ tp σ2a σ2c⌝))%I) →
+                                     ∗ (∀ σ2c, stateI σ2c ={⊤,E}=∗ φinv σ2c)))))%I) →
   crash_refines absr Λc ec (rec_singleton rec) (Λa.(exec) ea)
                 (and_then (Λa.(exec_halt) ea) (fun _ => Λa.(crash_step))).
 Proof.
-  intros Hsub Hwp_e Hwp_rec.
+  intros Hsub Hwp.
   assert (Hno_fault_cut :
             ∀ σ1a, ¬ (v <- exec Λa ea; _ <- absr; pure v) σ1a Err ->
                    ¬ exec Λa ea σ1a Err).
@@ -82,81 +80,66 @@ Proof.
              absr σ1a (Val σ1c tt) → recv_adequate NotStuck ec rec σ1c
                           (λ v' σ2c', ∃ σ2a, exec Λa ea σ1a (Val σ2a (existT _ v')) ∧
                                              absr σ2a (Val σ2c' tt))
-                          (λ σ2c', ∃ tp2 tp2' σ2a σ3a, pool_map_incl tp2 tp2' ∧
-                                                   exec_partial Λa ea σ1a (Val σ2a tp2') ∧
+                          (λ σ2c', ∃ tp2 σ2a σ3a, exec_partial Λa ea σ1a (Val σ2a tp2) ∧
                                                    crash_step Λa σ2a (Val σ3a tt) ∧
                                                    absr σ3a (Val σ2c' tt))).
-  { intros.
+  { intros σ1a σ1c ? Habsr_init.
     eapply wp_recovery_adequacy with
-        (φinv := fun σ2c => ∃ tp2 tp2' σ2a, pool_map_incl tp2 tp2' ∧ φ tp2 σ2a σ2c
-                                                ∧ exec_partial Λa ea σ1a (Val σ2a tp2')); eauto.
-    - iIntros (Hinv).
-      assert (Inhabited Λa.(State)).
-      { eexists; eauto. }
-      iMod (source_cfg_init [existT _ ea] σ1a) as (cfgG) "(#Hsrc&Hpool&HstateA)"; auto.
-      { intros Herr; apply Hno_fault. apply exec_partial_err_exec_err; eauto. }
-      iMod Hwp_e as (stateI) "Hwand"; eauto.
-      iDestruct ("Hwand" with "[Hpool HstateA]") as "[Hstate [H Hφ]]"; eauto.
-      { iFrame. iFrame "#".
-        rewrite /source_pool_map/tpool_to_map fmap_insert fmap_empty insert_empty //=.
-      }
-      iExists stateI. iIntros "{$Hstate} !>".
-      iSplitL "H".
-      * iApply wp_wand_l; iFrame "H". iIntros (v') "[Hmapsto Hopen]".
-        iIntros (σ2c') "Hstate".
-        iMod ("Hopen" with "Hstate") as (σ2a) "(Hstate&%)".
-        iInv "Hsrc" as (tp' σ') ">[Hauth Hp]" "_".
-        iDestruct "Hp" as %Hp. destruct Hp as (Hp&Hno_fault'). rewrite //= in Hp.
-        iDestruct (source_state_reconcile with "Hstate Hauth") as %Hstate; subst.
-        iDestruct (source_thread_reconcile with "Hmapsto Hauth") as %Hlookup; subst.
-        apply take_drop_middle in Hlookup.
+        (φinv0 := fun σ => (φinv σ ∗ ∃ _ : cfgG Σ, source_inv [existT T ea] σ1a)%I); eauto.
+    iIntros (Hinv).
+    assert (Inhabited Λa.(State)).
+    { eexists; eauto. }
+    iMod (source_cfg_init [existT _ ea] σ1a) as (cfgG) "(#Hsrc&Hpool&HstateA)"; auto.
+    { intros Herr; apply Hno_fault. apply exec_partial_err_exec_err; eauto. }
+    iPoseProof (Hwp _ _ Habsr_init $! Hinv cfgG) as "H".
+    iMod "H" as (stateI) "Hwand"; eauto.
+    iDestruct ("Hwand" with "[Hpool HstateA]") as "[Hstate [H [Hinv #Hφ]]]"; eauto.
+    { iFrame. iFrame "#".
+      rewrite /source_pool_map/tpool_to_map fmap_insert fmap_empty insert_empty //=.
+    }
+    iExists stateI. iIntros "{$Hstate} !>".
+    iSplitL "H"; last iSplitL "Hinv".
+    * iApply wp_wand_l; iFrame "H". iIntros (v') "[Hmapsto Hopen]".
+      iIntros (σ2c') "Hstate".
+      iMod ("Hopen" with "Hstate") as (σ2a) "(Hstate&%)".
+      iInv "Hsrc" as (tp' σ') ">[Hauth Hp]" "_".
+      iDestruct "Hp" as %Hp. destruct Hp as (Hp&Hno_fault'). rewrite //= in Hp.
+      iDestruct (source_state_reconcile with "Hstate Hauth") as %Hstate; subst.
+      iDestruct (source_thread_reconcile with "Hmapsto Hauth") as %Hlookup; subst.
+      apply take_drop_middle in Hlookup.
 
-        iApply fupd_mask_weaken; first by set_solver+.
-        iPureIntro. exists σ'; split; eauto.
-        rewrite -Hlookup //= /of_val in Hp.
-        eapply exec_partial_finish; eauto.
-      * iIntros (σ2c') "Hstate".
-        iMod ("Hφ" with "Hstate") as (tp2 σ2a) "(Hpool&Hstate&%)".
-        iInv "Hsrc" as (tp' σ') ">[Hauth Hp]" "_".
-        iDestruct "Hp" as %Hp. destruct Hp as (Hp&Hno_fault'). rewrite //= in Hp.
-        iDestruct (source_state_reconcile with "Hstate Hauth") as %Hstate; subst.
-        iDestruct (source_pool_map_reconcile with "Hpool Hauth") as %Hpool; subst.
-
-        iApply fupd_mask_weaken; first by set_solver+.
-        iPureIntro. exists tp2, tp', σ'; split; eauto.
-    - iIntros (Hinv).
-      assert (Inhabited Λa.(State)).
-      { eexists; eauto. }
-      intros σ2c σ2c' (tp2&tp2'&σ2a&Hincl&Hφ&Hexec_partial) Hcrash.
-      iMod (source_cfg_init tp2' σ2a) as (cfgG) "(#Hsrc&Hpool&HstateA)".
-      { intros Herr; apply Hno_fault. apply exec_partial_err_exec_err; eauto.
-        eapply bind_star_trans; eauto.
-      }
-      iMod Hwp_rec as (stateI) "Hwand"; eauto.
-      iDestruct ("Hwand" with "[$]") as "[Hstate [H Hφ]]"; eauto.
-      iExists stateI. iIntros "{$Hstate} !>".
-      iSplitL "H".
-      * iApply wp_wand_l; iFrame "H". iIntros (v) "Hopen".
-        iIntros (σ3c) "Hstate".
-        iMod ("Hopen" with "Hstate") as (σ2a' σ3a) "(Hstate&%)".
-        iInv "Hsrc" as (tp' σ') ">[Hauth Hp]" "_".
-        iDestruct "Hp" as %Hp. rewrite //= in Hp.
-        iDestruct (source_state_reconcile with "Hstate Hauth") as %Hstate; subst.
-
-        iApply fupd_mask_weaken; first by set_solver+.
-        iPureIntro. exists (tpool_to_map tp'), tp', σ', σ3a; split_and!; intuition eauto.
-        { apply pool_map_incl_alt; reflexivity. }
-        { eapply bind_star_trans; eauto. }
-      * iIntros (σ3c) "Hstate".
-        iMod ("Hφ" with "Hstate") as (tp3 σ3a) "(Hpool&Hstate&%)".
-        iInv "Hsrc" as (tp' σ') ">[Hauth Hp]" "_".
-        iDestruct "Hp" as %Hp. rewrite //= in Hp.
-        iDestruct (source_state_reconcile with "Hstate Hauth") as %Hstate; subst.
-        iDestruct (source_pool_map_reconcile with "Hpool Hauth") as %Hpool; subst.
-
-        iApply fupd_mask_weaken; first by set_solver+.
-        iPureIntro. exists tp3, tp', σ'; split_and!; intuition eauto.
-        { eapply bind_star_trans; eauto. }
+      iApply fupd_mask_weaken; first by set_solver+.
+      iPureIntro. exists σ'; split; eauto.
+      rewrite -Hlookup //= /of_val in Hp.
+      eapply exec_partial_finish; eauto.
+    * iIntros. iMod ("Hinv" with "[$]").
+      iMod (inv_open_timeless with "Hsrc") as "(?&_)"; first by eassumption.
+      iApply fupd_mask_weaken; auto.
+      { set_solver+. }
+      iFrame. iExists _; eauto.
+    * iModIntro. iIntros (????) "(?&Hinv)".
+      iDestruct "Hinv" as (cfgG') "HcfgInv".
+      iClear "Hsrc".
+      iMod ("Hφ" with "[//] [$]") as (stateI') "(Hstate&Hwp&Hinv)".
+      iMod (inv_alloc sourceN ⊤ (source_inv _ _) with "HcfgInv") as "#cfgInv".
+      iModIntro. iExists stateI'. iFrame.
+      iSplitL "Hwp".
+      ** iApply wp_wand_l; iFrame.
+         iIntros (_) "H1".
+         iIntros (σ) "Hstate".
+         iMod ("H1" with "[$]") as (σ2a σ3a) "(Hstate&Hp)".
+         iDestruct "Hp" as %(Hcrash&Habsr).
+         iMod (inv_open_timeless with "cfgInv") as "(Hinv&_)"; first by eassumption.
+         iApply fupd_mask_weaken; auto.
+         { set_solver+. }
+         iDestruct "Hinv" as (tp' σ3a') "(Hauth&%&%)".
+         iDestruct (source_state_reconcile with "Hstate Hauth") as %Hstate; subst.
+         iPureIntro. eexists _, _, _. intuition; eauto.
+      ** iIntros. iMod ("Hinv" with "[$]").
+         iMod (inv_open_timeless with "cfgInv") as "(?&_)"; first by eassumption.
+         iApply fupd_mask_weaken; auto.
+         { set_solver+. }
+         iFrame. iExists _; eauto.
   }
   split.
   - rewrite /refines.
@@ -188,7 +171,7 @@ Proof.
     }
     intros ([]&σ1c&Habsr&Hexec).
     edestruct Hadeq; eauto.
-    edestruct (recv_adequate_result) as (v'&?&σ2a&?&?&HexecA&HcrashA&Habsr'); eauto.
+    edestruct (recv_adequate_result) as (tp2&σ2a&?&HexecA&HcrashA&Habsr'); eauto.
     do 3 eexists; eauto.
     do 3 eexists; eauto.
     * unshelve (do 3 eexists; eauto); try exact tt.
@@ -200,7 +183,7 @@ Qed.
 Theorem wp_recovery_trace_refinement {T R} OpTa OpTc Σ (Λa: Layer OpTa) (Λc: Layer OpTc)
         `{invPreG Σ} `{cfgPreG OpTa Λa Σ}
         (ea: proc OpTa T) (ec: proc OpTc T) (rec: proc OpTc R)
-        φ (absr: relation Λa.(State) Λc.(State) unit) E
+        φinv (absr: relation Λa.(State) Λc.(State) unit) E
         (Habsr_no_err: ∀ σa, ¬ absr σa Err):
   nclose sourceN ⊆ E →
   (∀ (σ1a: Λa.(State)) σ1c,
@@ -208,31 +191,33 @@ Theorem wp_recovery_trace_refinement {T R} OpTa OpTc Σ (Λa: Layer OpTa) (Λc: 
       (∀ `{Hinv : invG Σ} `{Hcfg: cfgG OpTa Λa Σ},
           (|={⊤}=> ∃ stateI : State Λc → iProp Σ,
              let _ : irisG OpTc Λc Σ := IrisG _ _ _ Hinv stateI in
-             (source_ctx ([existT _ ea], σ1a) ∗ O ⤇ ea ∗ source_state σ1a) -∗
-              stateI σ1c ∗ WP ec @ NotStuck; ⊤ {{ v, O ⤇ of_val v
+             (source_ctx ([existT _ ea], σ1a) ∗ O ⤇ ea ∗ source_state σ1a)
+               -∗
+               stateI σ1c
+               ∗ WP ec @ NotStuck; ⊤ {{ v, O ⤇ of_val v
                     ∗ (∀ σ2c, stateI σ2c ={⊤,E}=∗ ∃ σ2a, source_state σ2a ∗ ⌜absr σ2a (Val σ2c tt)⌝)}}
-                              ∗ (∀ σ2c, stateI σ2c ={⊤,E}=∗ ∃ tp σ2a, source_pool_map tp
-                                         ∗ source_state σ2a ∗ ⌜φ tp σ2a σ2c⌝))%I)) →
-  (∀ `{Hinv : invG Σ} `{Hcfg: cfgG OpTa Λa Σ}
-     tp1 tp1' σ1a σ1c σ1c'
-     (Hφ: φ tp1 σ1a σ1c)
-     (Htp_sub: pool_map_incl tp1 tp1')
-     (Hcrash: Λc.(crash_step) σ1c (Val σ1c' tt)),
-     (|={⊤}=> ∃ stateI : State Λc → iProp Σ,
-       let _ : irisG OpTc Λc Σ := IrisG _ _ _ Hinv stateI in
-       (source_ctx (tp1', σ1a) ∗ source_pool_map (tpool_to_map tp1') ∗ source_state σ1a) -∗
-              stateI σ1c' ∗ WP rec @ NotStuck; ⊤ {{ v, (∀ σ2c, stateI σ2c ={⊤,E}=∗
-                     ∃ σ2a σ2a', source_state σ2a ∗ ⌜Λa.(crash_step) σ2a (Val σ2a' tt)
-                                 ∧ absr σ2a' (Val σ2c tt)⌝)}}
-                              ∗ (∀ σ2c, stateI σ2c ={⊤,E}=∗ ∃ tp σ2a, source_pool_map tp
-                                         ∗ source_state σ2a ∗ ⌜φ tp σ2a σ2c⌝))%I) →
-  (∀ tp σa σc, φ tp σa σc → trace_relation _ _ σa (Val σc tt)) →
+                                      ∗ (∀ σ2c, stateI σ2c ={⊤,E}=∗ φinv σ2c
+                                                ∗ ∃ σ2a, source_state σ2a
+                                                     ∗ ⌜ trace_relation _ _ σ2a (Val σ2c tt) ⌝)
+        ∗
+        □ (∀ `{Hinv : invG Σ} `{Hcfg: cfgG OpTa Λa Σ} σ1c σ1c'
+           (Hcrash: Λc.(crash_step) σ1c (Val σ1c' tt)),
+            (φinv σ1c ={⊤}=∗ ∃ stateI : State Λc → iProp Σ,
+               let _ : irisG OpTc Λc Σ := IrisG _ _ _ Hinv stateI in
+               stateI σ1c'
+               ∗ WP rec @ NotStuck; ⊤ {{ v, (∀ σ2c, stateI σ2c ={⊤,E}=∗
+                   ∃ σ2a σ2a', source_state σ2a ∗ ⌜Λa.(crash_step) σ2a (Val σ2a' tt)
+                               ∧ absr σ2a' (Val σ2c tt)⌝)}}
+                                      ∗ (∀ σ2c, stateI σ2c ={⊤,E}=∗ φinv σ2c
+                                                ∗ ∃ σ2a, source_state σ2a
+                                                     ∗ ⌜ trace_relation _ _ σ2a (Val σ2c tt) ⌝)))))%I)
+    →
   halt_refines absr Λc (trace_relation Λc Λa)
                  ec
                  (rec_singleton rec) (Λa.(exec_halt) ea)
                  (and_then (Λa.(exec_halt) ea) (fun _ => Λa.(crash_step))).
 Proof.
-  intros Hsub Hwp_e Hwp_rec Hφ_trace.
+  intros Hsub Hwp.
   apply halt_refines_trace_relation_alt; eauto.
   rewrite /halt_refines/refines_if.
   assert (Hno_fault_cut :
@@ -254,7 +239,7 @@ Proof.
   assert (∃ σ1c_outer,
              absr σ1a (Val σ1c_outer ()) ∧
              rexec_partial Λc ec (rec_singleton rec) σ1c_outer ret)
-         as (σ1c_outer&Habsr&Hexec).
+         as (σ1c_outer&Habsr_init&Hexec).
   {
     destruct ret.
     - destruct Hstep as ([]&?&?&?). eexists; split; eauto.
@@ -265,83 +250,96 @@ Proof.
   edestruct @wp_recovery_invariance with
         (ρ := fun σ2c => (v <- _ <- exec_halt Λa ea;
             Λa.(crash_step); _ <- trace_relation Λc Λa; pure v) σ1a (Val σ2c ()))
-        (φinv := fun σ2c => ∃ tp2 tp2' σ2a, pool_map_incl tp2 tp2' ∧ φ tp2 σ2a σ2c
-                                            ∧ exec_partial Λa ea σ1a (Val σ2a tp2'))
+        (φ := fun (_ : T) (_ : Λc.(State)) => True)
+        (φrec := fun (_ : Λc.(State)) => True)
+        (φinv := fun σ => (φinv σ ∗ ∃ _ : cfgG Σ, source_inv [existT T ea] σ1a)%I)
         as (Hρ&Hadeq); eauto.
-  - iIntros (Hinv).
+  {
+    iIntros (Hinv).
     assert (Inhabited Λa.(State)).
     { eexists; eauto. }
-    iMod (source_cfg_init [existT _ ea] σ1a) as (cfgG) "(#Hsrc&Hpool&HstateA)".
+    iMod (source_cfg_init [existT _ ea] σ1a) as (cfgG) "(#Hsrc&Hpool&HstateA)"; auto.
     { intros Herr. eapply Hno_fault_cut'; first eapply Hno_fault.
       apply exec_partial_err_exec_err; eauto. }
-    iMod Hwp_e as (stateI) "Hwand"; eauto.
-    iDestruct ("Hwand" with "[Hpool HstateA]") as "[Hstate [H Hφ]]"; eauto.
-    {
-      iFrame. iFrame "#".
+    iPoseProof (Hwp _ _ Habsr_init $! Hinv cfgG) as "H".
+    iMod "H" as (stateI) "Hwand"; eauto.
+    iDestruct ("Hwand" with "[Hpool HstateA]") as "[Hstate [H [Hinv #Hφ]]]"; eauto.
+    { iFrame. iFrame "#".
       rewrite /source_pool_map/tpool_to_map fmap_insert fmap_empty insert_empty //=.
     }
     iExists stateI. iIntros "{$Hstate} !>".
-    iSplitL "H".
-    * iApply wp_wand_l; iFrame "H"; auto.
-    * iIntros (σ2c') "Hstate".
-      iMod ("Hφ" with "Hstate") as (tp2 σ2a) "(Hpool&Hstate&%)".
+    iSplitL "H"; last iSplitL "Hinv".
+    * iApply wp_wand_l; iFrame "H". iIntros (v') "[Hmapsto Hopen]".
+      iIntros (σ2c') "Hstate".
+      iMod ("Hopen" with "Hstate") as (σ2a) "(Hstate&%)".
       iInv "Hsrc" as (tp' σ') ">[Hauth Hp]" "_".
       iDestruct "Hp" as %Hp. destruct Hp as (Hp&Hno_fault'). rewrite //= in Hp.
       iDestruct (source_state_reconcile with "Hstate Hauth") as %Hstate; subst.
-      iDestruct (source_pool_map_reconcile with "Hpool Hauth") as %Hpool; subst.
+      iDestruct (source_thread_reconcile with "Hmapsto Hauth") as %Hlookup; subst.
+      apply take_drop_middle in Hlookup.
 
       iApply fupd_mask_weaken; first by set_solver+.
-      iPureIntro. exists tp2, tp', σ'; split; eauto.
-  - iIntros (Hinv).
-    assert (Inhabited Λa.(State)).
-    { eexists; eauto. }
-    intros σ2c σ2c' (tp2&tp2'&σ2a&Hincl&Hφ&Hexec_partial) Hcrash.
-    iMod (source_cfg_init tp2' σ2a) as (cfgG) "(#Hsrc&Hpool&HstateA)".
-    { intros Herr. eapply Hno_fault_cut'; first eapply Hno_fault.
-      apply exec_partial_err_exec_err.
-      eapply bind_star_trans; eauto.
-    }
-    iMod Hwp_rec as (stateI) "Hwand"; eauto.
-    iDestruct ("Hwand" with "[$]") as "[Hstate [H Hφ]]"; eauto.
-    iExists stateI. iIntros "{$Hstate} !>".
-    iSplitL "H".
-    * iApply wp_wand_l; iFrame "H"; eauto.
-    * iIntros (σ3c) "Hstate".
-      iMod ("Hφ" with "Hstate") as (tp3 σ3a) "(Hpool&Hstate&%)".
-      iInv "Hsrc" as (tp' σ') ">[Hauth Hp]" "_".
-      iDestruct "Hp" as %Hp. rewrite //= in Hp.
+      iPureIntro; auto.
+    * iIntros.
+      iMod ("Hinv" with "[$]") as "(Hφinv&Hrest)".
+      iDestruct "Hrest" as (σ2a) "(Hstate&Htrace)". iDestruct "Htrace" as %Htrace.
+      iMod (inv_open_timeless with "Hsrc") as "(Hinv&_)"; first by eassumption.
+      iApply fupd_mask_weaken; auto.
+      { set_solver+. }
+      iDestruct "Hinv" as (tp' σ3a') "(Hauth&%&%)".
       iDestruct (source_state_reconcile with "Hstate Hauth") as %Hstate; subst.
-      iDestruct (source_pool_map_reconcile with "Hpool Hauth") as %Hpool; subst.
-
-      iApply fupd_mask_weaken; first by set_solver+.
-      iPureIntro. exists tp3, tp', σ'; split_and!; intuition eauto.
-      { eapply bind_star_trans; eauto. }
-  - intros σ (tp2&tp2'&σ2a&Hincl&?&Hexec').
-    edestruct (crash_total _ σ2a) as (σ2a'&?).
-    do 3 eexists.
-    { do 3 eexists; eauto.
-      do 3 eexists; eauto.
-      econstructor; eauto.
-    }
-    eexists tt, _; split; last by econstructor.
-    eexists; split; eauto.
-    transitivity (trace_proj _ σ2a).
-    { symmetry. eapply crash_preserves_trace; eauto. }
-    { edestruct Hφ_trace; intuition; eauto. inversion H4; subst. eauto. }
-  - intros σ1c σ2c (tp2&tp2'&σ2a&Hincl&Hφ&Hexec') Hcrash.
-    edestruct (crash_total _ σ2a) as (σ2a'&?).
-    do 3 eexists.
-    { do 3 eexists; eauto.
-      do 3 eexists; eauto.
-      econstructor; eauto.
-    }
-    eexists tt, _; split; last by econstructor.
-    eexists; split; eauto.
-    transitivity (trace_proj _ σ2a).
-    { symmetry. eapply crash_preserves_trace; eauto. }
-    transitivity (trace_proj _ σ1c).
-    { edestruct Hφ_trace; intuition; eauto. inversion H3; subst. eauto. }
-    { eapply crash_preserves_trace; eauto. }
-  - destruct ret as [? []|]; eauto.
-    exfalso. eapply recv_adequate_not_stuck; eauto using rexec_partial_err_rexec_err.
+      iFrame. iSplit.
+      ** iExists _, _; eauto.
+      ** iPureIntro.
+         edestruct (crash_total _ σ3a') as (σ3a''&?).
+         do 3 eexists.
+         { do 3 eexists; eauto.
+           do 3 eexists; eauto.
+           econstructor; eauto.
+         }
+         eexists tt, _; split; last by econstructor.
+         eexists; split; eauto.
+         transitivity (trace_proj _ σ3a').
+         { symmetry. eapply crash_preserves_trace; eauto. }
+         { inversion Htrace as (?&Heq&?). inversion Heq; subst; eauto. }
+    * iModIntro. iIntros (????) "(?&Hinv)".
+      iDestruct "Hinv" as (cfgG') "HcfgInv".
+      iClear "Hsrc".
+      iMod ("Hφ" with "[//] [$]") as (stateI') "(Hstate&Hwp&Hinv)".
+      iMod (inv_alloc sourceN ⊤ (source_inv _ _) with "HcfgInv") as "#cfgInv".
+      iModIntro. iExists stateI'. iFrame.
+      iSplitL "Hwp".
+      ** iApply wp_wand_l; iFrame.
+         iIntros (_) "H1".
+         iIntros (σ) "Hstate".
+         iMod ("H1" with "[$]") as (σ2a σ3a) "(Hstate&Hp)".
+         iDestruct "Hp" as %(Hcrash&Habsr).
+         iMod (inv_open_timeless with "cfgInv") as "(Hinv&_)"; first by eassumption.
+         iApply fupd_mask_weaken; auto.
+         { set_solver+. }
+      ** iIntros.
+         iMod ("Hinv" with "[$]") as "(Hφinv&Hrest)".
+         iDestruct "Hrest" as (σ2a) "(Hstate&Htrace)". iDestruct "Htrace" as %Htrace.
+         iMod (inv_open_timeless with "cfgInv") as "(Hinv&_)"; first by eassumption.
+         iApply fupd_mask_weaken; auto.
+         { set_solver+. }
+         iDestruct "Hinv" as (tp' σ3a') "(Hauth&%&%)".
+         iDestruct (source_state_reconcile with "Hstate Hauth") as %Hstate; subst.
+         iFrame. iSplit.
+         *** iExists _, _; eauto.
+         *** iPureIntro.
+         edestruct (crash_total _ σ3a') as (σ3a''&?).
+         do 3 eexists.
+         { do 3 eexists; eauto.
+           do 3 eexists; eauto.
+           econstructor; eauto.
+         }
+         eexists tt, _; split; last by econstructor.
+         eexists; split; eauto.
+         transitivity (trace_proj _ σ3a').
+         { symmetry. eapply crash_preserves_trace; eauto. }
+         { inversion Htrace as (?&Heq&?). inversion Heq; subst; eauto. }
+  }
+  destruct ret as [? []|]; eauto.
+  exfalso. eapply recv_adequate_not_stuck; eauto using rexec_partial_err_rexec_err.
 Qed.
